generating the top-level theorems.
git-svn-id: https://webdav.seas.upenn.edu/svn/sol/vol@3657 eef5ea85-cc2e-0410-bd84-0fae1f012da8

src/Transforms/palloca_props.v
@@ -23,6 +23,7 @@ Record PhiInfo := mkPhiInfo {
   PI_preds: ATree.t (list l);
   PI_id: id;
   PI_typ: typ;
+  PI_num: value;
   PI_align: align;
   PI_newids: ATree.t (id*id*id)  
 }.
