src/Transforms/die.v
@@ -1,0 +1,151 @@
+Add LoadPath "../Vellvm/ott".
+Add LoadPath "../Vellvm/monads".
+Add LoadPath "../Vellvm/compcert".
+Add LoadPath "../Vellvm/GraphBasics".
+Add LoadPath "../Vellvm".
+Add LoadPath "../../../theory/metatheory_8.3".
+Add LoadPath "../SoftBound".
+Require Import vellvm.
+Require Import Kildall.
+Require Import ListSet.
+Require Import Maps.
+Require Import Lattice.
+Require Import Iteration.
+Require Import Maps.
+Require Import opsem_props.
+Require Import primitives.
+
+Definition pure_cmd (c:cmd) : Prop :=
+match c with
+| insn_alloca _ _ _ _  
+| insn_malloc _ _ _ _  
+| insn_store _ _ _ _ _
+| insn_call _ _ _ _ _ _ => False
+| _ => True
+end.
+
+Record DIInfo := mkDIInfo {
+  DI_f : fdef;
+  DI_id : id;
+  DI_pure : forall c, 
+               lookupInsnViaIDFromFdef DI_f DI_id = Some (insn_cmd c) -> 
+               pure_cmd c;
+  DI_unused : used_in_fdef DI_id DI_f = false
+}.
+
+Definition fdef_simulation (diinfo: DIInfo) f1 f2 : Prop :=
+  if (fdef_dec (DI_f diinfo) f1) then remove_fdef (DI_id diinfo) f1 = f2
+  else f1 = f2.
+
+Definition cmds_simulation (diinfo: DIInfo) (f1:fdef) cs1 cs2 : Prop :=         
+  if (fdef_dec (DI_f diinfo) f1) then remove_cmds (DI_id diinfo) cs1 = cs2
+  else cs1 = cs2.
+
+Definition block_simulation (diinfo: DIInfo) (f1:fdef) b1 b2 : Prop :=
+  if (fdef_dec (DI_f diinfo) f1) then remove_block (DI_id diinfo) b1 = b2
+  else b1 = b2.
+
+Definition products_simulation (diinfo: DIInfo) Ps1 Ps2 : Prop :=
+List.Forall2 
+  (fun P1 P2 =>
+   match P1, P2 with
+   | product_fdef f1, product_fdef f2 => fdef_simulation diinfo f1 f2
+   | _, _ => P1 = P2
+   end) Ps1 Ps2.
+
+Definition system_simulation (diinfo: DIInfo) S1 S2 : Prop :=
+List.Forall2 
+  (fun M1 M2 =>
+   match M1, M2 with
+   | module_intro los1 nts1 Ps1, module_intro los2 nts2 Ps2 =>
+       los1 = los2 /\ nts1 = nts2 /\ 
+       products_simulation diinfo Ps1 Ps1
+   end) S1 S2.
+
+Definition reg_simulation (diinfo: DIInfo) (F1:fdef) 
+  (lc1 lc2:@Opsem.GVsMap DGVs) : Prop :=
+  if (fdef_dec (DI_f diinfo) F1) then 
+    forall i0, i0 <> DI_id diinfo -> lookupAL _ lc1 i0 = lookupAL _ lc2 i0
+  else
+    lc1 = lc2.
+
+Definition EC_simulation (diinfo: DIInfo) (EC1 EC2:@Opsem.ExecutionContext DGVs) 
+  : Prop :=
+  match (EC1, EC2) with
+  | (Opsem.mkEC f1 b1 cs1 tmn1 lc1 als1, 
+     Opsem.mkEC f2 b2 cs2 tmn2 lc2 als2) =>
+       fdef_simulation diinfo f1 f2 /\
+       tmn1 = tmn2 /\
+       als1 = als2 /\
+       block_simulation diinfo f1 b1 b2 /\
+       (exists l1, exists ps1, exists cs11, 
+         b1 = block_intro l1 ps1 (cs11++cs1) tmn1)
+         /\
+       (exists l2, exists ps2, exists cs21,
+         b2 = block_intro l2 ps2 (cs21++cs2) tmn2) /\
+       reg_simulation diinfo f1 lc1 lc2 /\
+       cmds_simulation diinfo f1 cs1 cs2
+  end.
+
+Fixpoint ECs_simulation (diinfo: DIInfo) (ECs1 ECs2:@Opsem.ECStack DGVs) 
+  : Prop :=
+match ECs1, ECs2 with
+| nil, nil => True
+| EC1::ECs1', EC2::ECs2' => 
+    EC_simulation diinfo EC1 EC2 /\ ECs_simulation diinfo ECs1' ECs2'
+| _, _ => False
+end.
+
+Definition State_simulation (diinfo: DIInfo)
+  (Cfg1:OpsemAux.Config) (St1:Opsem.State) 
+  (Cfg2:OpsemAux.Config) (St2:Opsem.State) : Prop :=
+let '(OpsemAux.mkCfg S1 TD1 Ps1 gl1 fs1) := Cfg1 in
+let '(OpsemAux.mkCfg S2 TD2 Ps2 gl2 fs2) := Cfg2 in
+match (St1, St2) with
+| (Opsem.mkState ECs1 M1, Opsem.mkState ECs2 M2) =>
+    TD1 = TD2 /\ 
+    products_simulation diinfo Ps1 Ps2 /\
+    ECs_simulation diinfo ECs1 ECs2 /\
+    gl1 = gl2 /\ fs1 = fs2 /\ M1 = M2
+end.
+
+Definition removable_State (diinfo: DIInfo) (St:@Opsem.State DGVs) : Prop :=
+match St with
+| Opsem.mkState
+    (Opsem.mkEC f b (c :: cs) tmn lc als::_) _ => 
+    if (fdef_dec (DI_f diinfo) f) then 
+      if (id_dec (DI_id diinfo) (getCmdLoc c)) then True else False
+    else False
+| _ => False
+end.
+
+Lemma removable_State_dec : forall diinfo St,
+  removable_State diinfo St \/ ~ removable_State diinfo St.
+Proof.
+  destruct St. 
+  destruct ECS as [|[]]; auto.
+  destruct CurCmds; auto.
+  simpl.
+  destruct (fdef_dec (DI_f diinfo) CurFunction); auto.
+  destruct (id_dec (DI_id diinfo) (getCmdLoc c)); auto.
+Qed.
+
+Lemma die_is_sim : forall diinfo Cfg1 St1 Cfg2 St2
+  (Hwfpp: OpsemPP.wf_State Cfg1 St1) 
+  (Hsim: State_simulation diinfo Cfg1 St1 Cfg2 St2),
+  (forall (Hrem: removable_State diinfo St1) St1' tr1 
+     (Hop1: Opsem.sInsn Cfg1 St1 St1' tr1), 
+      State_simulation diinfo Cfg1 St1' Cfg2 St2 /\ tr1 = trace_nil) /\
+  (forall (Hnrem: ~removable_State diinfo St1) St1' St2' tr1 tr2
+     (Hop2: Opsem.sInsn Cfg2 St2 St2' tr2) 
+     (Hop1: Opsem.sInsn Cfg1 St1 St1' tr1), 
+     State_simulation diinfo Cfg1 St1' Cfg2 St2' /\ tr1 = tr2).
+Admitted.
+
+(*****************************)
+(*
+*** Local Variables: ***
+*** coq-prog-name: "coqtop" ***
+*** coq-prog-args: ("-emacs-U" "-I" "~/SVN/sol/vol/src/Vellvm/monads" "-I" "~/SVN/sol/vol/src/Vellvm/ott" "-I" "~/SVN/sol/vol/src/Vellvm/compcert" "-I" "~/SVN/sol/theory/metatheory_8.3" "-impredicative-set") ***
+*** End: ***
+ *)
