src/Transforms/mem2reg_correct.v
@@ -1,0 +1,159 @@
+Add LoadPath "../Vellvm/ott".
+Add LoadPath "../Vellvm/monads".
+Add LoadPath "../Vellvm/compcert".
+Add LoadPath "../Vellvm/GraphBasics".
+Add LoadPath "../Vellvm".
+Add LoadPath "../../../theory/metatheory_8.3".
+Require Import vellvm.
+Require Import Kildall.
+Require Import ListSet.
+Require Import Maps.
+Require Import Lattice.
+Require Import Iteration.
+Require Import Maps.
+Require Import opsem_props.
+Require Import promotable_props.
+Require Import primitives.
+Require Import palloca_props.
+Require Import mem2reg.
+Require Import memory_props.
+
+(* opsem should use this definition *)
+Definition s_isFinialState (cfg:OpsemAux.Config) (state:@Opsem.State DGVs) 
+  : option GenericValue :=
+match state with
+| (Opsem.mkState ((Opsem.mkEC _ _ nil (insn_return_void _) _ _)::nil) _ ) => 
+    const2GV (OpsemAux.CurTargetData cfg) (OpsemAux.Globals cfg) 
+      (const_int Size.One (INTEGER.of_Z 1%Z 1%Z false))
+| (Opsem.mkState ((Opsem.mkEC _ _ nil (insn_return _ _ v) lc _)::nil) _ ) => 
+    Opsem.getOperandValue (OpsemAux.CurTargetData cfg) v lc 
+      (OpsemAux.Globals cfg)
+| _ => None
+end.
+
+(* opsem should use this definition *)
+Inductive s_converges : 
+  system -> id -> list (GVsT DGVs) -> trace -> GenericValue -> Prop :=
+| s_converges_intro : forall (s:system) (main:id) (VarArgs:list (GVsT DGVs))    
+                              cfg (IS FS:Opsem.State) r tr,
+  Opsem.s_genInitState s main VarArgs Mem.empty = Some (cfg, IS) ->
+  Opsem.sop_star cfg IS FS tr ->
+  s_isFinialState cfg FS = Some r ->
+  s_converges s main VarArgs tr r
+.
+
+Definition stuck_state (cfg:OpsemAux.Config) (st:@Opsem.State DGVs) : Prop :=
+~ exists st', exists tr, Opsem.sInsn cfg st st' tr.
+
+(* opsem should use this definition *)
+Inductive s_goeswrong : 
+  system -> id -> list (GVsT DGVs) -> trace -> @Opsem.State DGVs  -> Prop :=
+| s_goeswrong_intro : forall (s:system) (main:id) (VarArgs:list (GVsT DGVs)) 
+                              cfg (IS FS:Opsem.State) tr,
+  Opsem.s_genInitState s main VarArgs Mem.empty = Some (cfg, IS) ->
+  Opsem.sop_star cfg IS FS tr ->
+  stuck_state cfg FS ->
+  ~ Opsem.s_isFinialState FS ->
+  s_goeswrong s main VarArgs tr FS
+.
+
+Inductive program_sim (P1 P2:system) (main:id) (VarArgs:list (GVsT DGVs)) :
+   Prop :=
+| program_sim_intro: 
+    (forall tr r, 
+      s_converges P1 main VarArgs tr r -> 
+      s_converges P2 main VarArgs tr r) -> 
+    (forall Tr, 
+      Opsem.s_diverges P1 main VarArgs Tr -> 
+      Opsem.s_diverges P2 main VarArgs Tr) ->
+    program_sim P1 P2 main VarArgs
+.
+
+(* We are proving the macro-based m2r pass *)
+Axiom does_macro_m2r_is_true: mem2reg.does_macro_m2r tt = true.
+
+Lemma macro_m2r_sim_aux: forall (main : id) (VarArgs : list (GVsT DGVs))        
+  (los : layouts) (nts : namedts) (Ps2 Ps1: products),
+  program_sim
+    [module_intro los nts
+      (Ps1 ++ List.map
+        (fun p : product =>
+          match p with
+          | product_gvar _ => p
+          | product_fdec _ => p
+          | product_fdef f => product_fdef (mem2reg_fdef f)
+          end) Ps2)] [module_intro los nts (Ps1++Ps2)] main VarArgs.
+Proof.
+  induction Ps2; simpl; intros.
+    admit. (* refl *)
+
+    assert (J:=@IHPs2 (Ps1 ++ [a])). clear IHPs2.
+    simpl_env in J. simpl in J. 
+    destruct a; auto.
+
+
+
+  rewrite_env (nil ++ Ps) at 2.
+  rewrite_env (nil ++ List.map
+                (fun p : product =>
+                 match p with
+                 | product_gvar _ => p
+                 | product_fdec _ => p
+                 | product_fdef f => product_fdef (mem2reg_fdef f)
+                 end)).
+
+macro_m2r_sim_aux
+
+
+  destruct m as [los nts Ps].
+  intros.
+  constructor.
+    intros tr r Hconv.
+    inv Hconv.
+    unfold Opsem.s_genInitState in H.
+    inv_mbind'.
+    remember (productInModuleB_dec (product_fdef f)
+                (module_intro los nts
+                   (List.map
+                      (fun p : product =>
+                       match p with
+                       | product_gvar _ => p
+                       | product_fdec _ => p
+                       | product_fdef f => product_fdef (mem2reg_fdef f)
+                       end) Ps))) as R.
+    destruct R; inv HeqR0.
+    remember (OpsemAux.genGlobalAndInitMem
+           (OpsemAux.initTargetData los nts Mem.empty)
+           (List.map
+              (fun p : product =>
+               match p with
+               | product_gvar _ => p
+               | product_fdec _ => p
+               | product_fdef f => product_fdef (mem2reg_fdef f)
+               end) Ps) nil nil Mem.empty) as R.
+    destruct R as [[[initGlobal initFunTable] initMem]|]; inv H2.
+    inv_mbind'.
+    destruct b.
+    destruct f as [[]].
+    inv_mbind'. symmetry_ctx.
+
+    constructor.
+Qed.
+
+Lemma macro_m2r_sim: forall (m:module) (main:id) (VarArgs:list (GVsT DGVs)),
+  program_sim [mem2reg.run m] [m] main VarArgs.
+Proof.
+  destruct m as [los nts Ps].
+  unfold mem2reg.run.
+  intros.
+  assert (J:=@macro_m2r_sim_aux main VarArgs los nts Ps nil).
+  auto.
+Qed.
+
+(*****************************)
+(*
+*** Local Variables: ***
+*** coq-prog-name: "coqtop" ***
+*** coq-prog-args: ("-emacs-U" "-I" "~/SVN/sol/vol/src/Vellvm/monads" "-I" "~/SVN/sol/vol/src/Vellvm/ott" "-I" "~/SVN/sol/vol/src/Vellvm/compcert" "-I" "~/SVN/sol/theory/metatheory_8.3" "-impredicative-set") ***
+*** End: ***
+ *)
