src/Transforms/sas.v
@@ -1,0 +1,204 @@
+Add LoadPath "../Vellvm/ott".
+Add LoadPath "../Vellvm/monads".
+Add LoadPath "../Vellvm/compcert".
+Add LoadPath "../Vellvm/GraphBasics".
+Add LoadPath "../Vellvm".
+Add LoadPath "../../../theory/metatheory_8.3".
+Require Import vellvm.
+Require Import Kildall.
+Require Import ListSet.
+Require Import Maps.
+Require Import Lattice.
+Require Import Iteration.
+Require Import Maps.
+Require Import opsem_props.
+Require Import promotable_props.
+Require Import primitives.
+Require Import id_rhs_val.
+Require Import palloca_props.
+Require Import memory_props.
+
+Definition load_in_cmd (id':id) (c:cmd) : bool :=
+match c with
+| insn_load _ _ ptr _ => used_in_value id' ptr
+| _ => false
+end.
+
+Definition load_in_cmds (id':id) (cs:cmds) : bool := 
+(List.fold_left (fun re c => re || load_in_cmd id' c) cs false).
+
+Definition sas (sid1 sid2: id) (v1 v2:value) (cs2:cmds) (b:block) 
+  (pinfo:PhiInfo) : Prop :=         
+blockInFdefB b (PI_f pinfo) = true /\
+load_in_cmds (PI_id pinfo) cs2 = false /\
+let '(block_intro _ _ cs _) := b in
+exists cs1, exists cs3,
+  cs = 
+  cs1 ++ 
+  insn_store sid1 (PI_typ pinfo) v1 (value_id (PI_id pinfo)) (PI_align pinfo) ::
+  cs2 ++ 
+  insn_store sid2 (PI_typ pinfo) v2 (value_id (PI_id pinfo)) (PI_align pinfo) ::
+  cs3.
+
+Record SASInfo (pinfo: PhiInfo) := mkSASInfo {
+  SAS_sid1 : id;
+  SAS_sid2 : id;
+  SAS_value1 : value;
+  SAS_value2 : value;
+  SAS_tail : cmds;
+  SAS_block : block;
+  SAS_prop: sas SAS_sid1 SAS_sid2 SAS_value1 SAS_value2 SAS_tail SAS_block pinfo
+}.
+
+Definition fdef_simulation (pinfo: PhiInfo) (sasinfo: SASInfo pinfo) f1 f2 
+  : Prop :=
+  if (fdef_dec (PI_f pinfo) f1) then 
+    remove_fdef (SAS_sid1 pinfo sasinfo) f1 = f2
+  else f1 = f2.
+
+Definition cmds_simulation (pinfo: PhiInfo) (sasinfo: SASInfo pinfo) (f1:fdef) 
+  cs1 cs2 : Prop :=
+  if (fdef_dec (PI_f pinfo) f1) then 
+    remove_cmds (SAS_sid1 pinfo sasinfo) cs1 = cs2
+  else cs1 = cs2.
+
+Definition block_simulation (pinfo: PhiInfo) (sasinfo: SASInfo pinfo) (f1:fdef) 
+  b1 b2 : Prop :=
+  if (fdef_dec (PI_f pinfo) f1) then 
+    remove_block (SAS_sid1 pinfo sasinfo) b1 = b2
+  else b1 = b2.
+
+Definition products_simulation (pinfo: PhiInfo) (sasinfo: SASInfo pinfo) Ps1 Ps2
+  : Prop :=
+List.Forall2 
+  (fun P1 P2 =>
+   match P1, P2 with
+   | product_fdef f1, product_fdef f2 => fdef_simulation pinfo sasinfo f1 f2
+   | _, _ => P1 = P2
+   end) Ps1 Ps2.
+
+Definition system_simulation (pinfo: PhiInfo) (sasinfo: SASInfo pinfo) S1 S2 
+  : Prop :=
+List.Forall2 
+  (fun M1 M2 =>
+   match M1, M2 with
+   | module_intro los1 nts1 Ps1, module_intro los2 nts2 Ps2 =>
+       los1 = los2 /\ nts1 = nts2 /\ 
+       products_simulation pinfo sasinfo Ps1 Ps1
+   end) S1 S2.
+
+Definition EC_simulation (pinfo: PhiInfo) (sasinfo: SASInfo pinfo) 
+  (EC1 EC2:@Opsem.ExecutionContext DGVs) : Prop :=
+  match (EC1, EC2) with
+  | (Opsem.mkEC f1 b1 cs1 tmn1 lc1 als1, 
+     Opsem.mkEC f2 b2 cs2 tmn2 lc2 als2) =>
+       fdef_simulation pinfo sasinfo f1 f2 /\
+       tmn1 = tmn2 /\
+       als1 = als2 /\
+       block_simulation pinfo sasinfo f1 b1 b2 /\
+       (exists l1, exists ps1, exists cs11, 
+         b1 = block_intro l1 ps1 (cs11++cs1) tmn1)
+         /\
+       (exists l2, exists ps2, exists cs21,
+         b2 = block_intro l2 ps2 (cs21++cs2) tmn2) /\
+       lc1 = lc2 /\
+       cmds_simulation pinfo sasinfo f1 cs1 cs2
+  end.
+
+Fixpoint ECs_simulation (pinfo: PhiInfo) (sasinfo: SASInfo pinfo) 
+  (ECs1 ECs2:@Opsem.ECStack DGVs) : Prop :=
+match ECs1, ECs2 with
+| nil, nil => True
+| EC1::ECs1', EC2::ECs2' => 
+    EC_simulation pinfo sasinfo EC1 EC2 /\ 
+    ECs_simulation pinfo sasinfo ECs1' ECs2'
+| _, _ => False
+end.
+
+Definition cs_follow_dead_store (pinfo:PhiInfo) (sasinfo: SASInfo pinfo)
+  (cs:cmds) : Prop :=
+let '(block_intro _ _ cs0 _) := SAS_block pinfo sasinfo in
+forall cs1 cs3, 
+  cs0 = 
+    cs1 ++ 
+    insn_store (SAS_sid1 pinfo sasinfo) (PI_typ pinfo) 
+      (SAS_value1 pinfo sasinfo) (value_id (PI_id pinfo)) (PI_align pinfo) ::
+    SAS_tail pinfo sasinfo ++ 
+    cs3 ->
+  (exists csa, exists csb, 
+    cs = csb ++ cs3 /\ SAS_tail pinfo sasinfo = csa ++ csb).
+
+Definition EC_follow_dead_store (pinfo:PhiInfo) (sasinfo: SASInfo pinfo)
+  (ec:@Opsem.ExecutionContext DGVs) : Prop :=
+Opsem.CurFunction ec = PI_f pinfo /\
+Opsem.CurBB ec = SAS_block pinfo sasinfo /\
+cs_follow_dead_store pinfo sasinfo (Opsem.CurCmds ec).
+
+Definition undead_head_in_tail (pinfo:PhiInfo) (sasinfo: SASInfo pinfo) ptr
+  (ec0:@Opsem.ExecutionContext DGVs) : Prop :=
+forall gvsa (Heq: Opsem.CurFunction ec0 = PI_f pinfo)
+  (Hlkup: lookupAL _ (Opsem.Locals ec0) (PI_id pinfo) = Some gvsa),
+  MemProps.no_alias ptr gvsa \/
+  ~ MemProps.no_alias ptr gvsa /\ EC_follow_dead_store pinfo sasinfo ec0.
+
+Definition undead_head_tail (pinfo:PhiInfo) (sasinfo: SASInfo pinfo) ptr 
+  (ecs':list Opsem.ExecutionContext) : Prop :=
+  forall ec0 (Hin: In ec0 ecs'), undead_head_in_tail pinfo sasinfo ptr ec0.
+
+Definition Mem_simulation (pinfo:PhiInfo) (sasinfo: SASInfo pinfo) TD 
+  (ecs1:list Opsem.ExecutionContext) Mem1 Mem2 : Prop :=
+Mem.nextblock Mem1 = Mem.nextblock Mem2 /\
+forall ptr ty al gvs1 gvs2 
+  (Hnalias: undead_head_tail pinfo sasinfo ptr ecs1)
+  (Hld1: mload TD Mem1 ptr ty al = Some gvs1)
+  (Hld2: mload TD Mem2 ptr ty al = Some gvs2),
+  gvs1 = gvs2.
+
+Definition State_simulation (pinfo: PhiInfo) (sasinfo: SASInfo pinfo) 
+  (Cfg1:OpsemAux.Config) (St1:Opsem.State) 
+  (Cfg2:OpsemAux.Config) (St2:Opsem.State) : Prop :=
+let '(OpsemAux.mkCfg S1 TD1 Ps1 gl1 fs1) := Cfg1 in
+let '(OpsemAux.mkCfg S2 TD2 Ps2 gl2 fs2) := Cfg2 in
+match (St1, St2) with
+| (Opsem.mkState ECs1 M1, Opsem.mkState ECs2 M2) =>
+    TD1 = TD2 /\ 
+    products_simulation pinfo sasinfo Ps1 Ps2 /\
+    ECs_simulation pinfo sasinfo ECs1 ECs2 /\
+    gl1 = gl2 /\ fs1 = fs2 /\ Mem_simulation pinfo sasinfo TD1 ECs1 M1 M2
+end.
+
+Definition removable_State (pinfo: PhiInfo) (sasinfo: SASInfo pinfo) 
+  (St:@Opsem.State DGVs) : Prop :=
+match St with
+| Opsem.mkState
+    (Opsem.mkEC f b 
+      (insn_store sid _ _ _ _ :: cs) 
+      tmn lc als::_) _ => 
+    if (fdef_dec (PI_f pinfo) f) then 
+      if (id_dec sid (SAS_sid1 pinfo sasinfo)) 
+      then True else False
+    else False
+| _ => False
+end.
+
+Lemma dse_is_sim : forall maxb pinfo (sasinfo: SASInfo pinfo) Cfg1 St1 Cfg2 St2
+  (Hwfpi: WF_PhiInfo pinfo) 
+  (Hwfpp: OpsemPP.wf_State Cfg1 St1) 
+  (Hnoalias: Promotability.wf_State maxb pinfo Cfg1 St1) 
+  (Hsim: State_simulation pinfo sasinfo Cfg1 St1 Cfg2 St2),
+  (forall (Hrem: removable_State pinfo sasinfo St1) St1' tr1 
+     (Hop1: Opsem.sInsn Cfg1 St1 St1' tr1), 
+     State_simulation pinfo sasinfo Cfg1 St1' Cfg2 St2 /\ tr1 = trace_nil) /\
+  (forall (Hnrem: ~removable_State pinfo sasinfo St1) St1' St2' tr1 tr2
+     (Hop2: Opsem.sInsn Cfg2 St2 St2' tr2) 
+     (Hop1: Opsem.sInsn Cfg1 St1 St1' tr1), 
+     State_simulation pinfo sasinfo Cfg1 St1' Cfg2 St2' /\ tr1 = tr2).
+Admitted.
+
+(*****************************)
+(*
+*** Local Variables: ***
+*** coq-prog-name: "coqtop" ***
+*** coq-prog-args: ("-emacs-U" "-I" "~/SVN/sol/vol/src/Vellvm/monads" "-I" "~/SVN/sol/vol/src/Vellvm/ott" "-I" "~/SVN/sol/vol/src/Vellvm/compcert" "-I" "~/SVN/sol/theory/metatheory_8.3" "-impredicative-set") ***
+*** End: ***
+ *)
